NLustreToSyBloc/Correctness.v
@@ -99,53 +99,54 @@ Module Type CORRECTNESS
       Forall (msem_equation G bk H M M') (n_eqs n) ->
       reset_lasts (translate_node n) (M 0).
   Proof.
-    intros ** Closed Heqs ?? Hin.
-    destruct n; simpl in *.
-    unfold gather_eqs in *.
-    clear - Heqs Hin.
-    revert Hin; generalize (@nil (ident * ident)).
-    induction n_eqs0 as [|[] ? IH]; simpl in *; intros; try contradiction;
-      inversion_clear Heqs as [|?? Heq]; inv Heq; eauto.
-    + destruct i; try discriminate; eauto.
-    + destruct i; try discriminate; eauto.
-    + apply In_fst_fold_left_gather_eq in Hin as [Hin|]; eauto.
-      destruct Hin as [E|]; try contradiction; inv E.
-      match goal with H: mfby _ _ _ _ _ _ |- _ => destruct H as (?&?) end; auto.
-    (*   intros ** Closed Heqs. *)
-    (* split. *)
-    (* - intros ** Hin. *)
-    (*   destruct n; simpl in *. *)
-    (*   unfold gather_eqs in *. *)
-    (*   clear - Heqs Hin. *)
-    (*   revert Hin; generalize (@nil (ident * ident)). *)
-    (*   induction n_eqs0 as [|[] ? IH]; simpl in *; intros; try contradiction; *)
-    (*     inversion_clear Heqs as [|?? Heq]; inv Heq; eauto. *)
-    (*   + destruct i; try discriminate; eauto. *)
-    (*   + destruct i; try discriminate; eauto. *)
-    (*   + apply In_fst_fold_left_gather_eq in Hin as [Hin|]; eauto. *)
-    (*     destruct Hin as [E|]; try contradiction; inv E. *)
-    (*     match goal with H: mfby _ _ _ _ _ _ |- _ => destruct H as (?&?) end; auto. *)
-    (* - specialize (Closed 0); destruct Closed as [? Vals]. *)
-    (*   intros ** Find. *)
-    (*   assert (In x (SynNL.gather_mem (n_eqs n))) as Hin *)
-    (*       by (apply Vals, not_None_is_Some; eauto). *)
-    (*   destruct n; simpl in *. *)
-    (*   unfold gather_eqs in *. *)
-    (*   clear - Hin Find Heqs. *)
-    (*   revert Hin; generalize (@nil (ident * ident)). *)
-    (*   induction n_eqs0 as [|[] ? IH]; simpl in *; intros; try contradiction; *)
-    (*     inversion_clear Heqs as [|?? Heq]; inv Heq; eauto. *)
-    (*   + destruct i; try discriminate; eauto. *)
-    (*   + destruct i; try discriminate; eauto. *)
-    (*   + destruct Hin. *)
-    (*     * subst. *)
-    (*       match goal with H: mfby _ _ _ _ _ _ |- _ => destruct H as (Find'&?) end. *)
-    (*       rewrite Find in Find'; inv Find'. *)
-    (*       exists c0; split; auto. *)
-    (*       apply In_fst_fold_left_gather_eq; left; left; auto. *)
-    (*     * edestruct IH as (c1 &?& Hin); eauto. *)
-    (*       exists c1; split; auto. *)
-    (*       apply In_fst_fold_left_gather_eq; right; eauto. *)
+    (* intros ** Closed Heqs ?? Hin. *)
+    (* destruct n; simpl in *. *)
+    (* unfold gather_eqs in *. *)
+    (* clear - Heqs Hin. *)
+    (* revert Hin; generalize (@nil (ident * ident)). *)
+    (* induction n_eqs0 as [|[] ? IH]; simpl in *; intros; try contradiction; *)
+    (*   inversion_clear Heqs as [|?? Heq]; inv Heq; eauto. *)
+    (* + destruct i; try discriminate; eauto. *)
+    (* + destruct i; try discriminate; eauto. *)
+    (* + apply In_fst_fold_left_gather_eq in Hin as [Hin|]; eauto. *)
+    (*   destruct Hin as [E|]; try contradiction; inv E. *)
+    (*   match goal with H: mfby _ _ _ _ _ _ |- _ => destruct H as (?&?) end; auto. *)
+
+    intros ** Closed Heqs.
+    split.
+    - intros ** Hin.
+      destruct n; simpl in *.
+      unfold gather_eqs in *.
+      clear - Heqs Hin.
+      revert Hin; generalize (@nil (ident * ident)).
+      induction n_eqs0 as [|[] ? IH]; simpl in *; intros; try contradiction;
+        inversion_clear Heqs as [|?? Heq]; inv Heq; eauto.
+      + destruct i; try discriminate; eauto.
+      + destruct i; try discriminate; eauto.
+      + apply In_fst_fold_left_gather_eq in Hin as [Hin|]; eauto.
+        destruct Hin as [E|]; try contradiction; inv E.
+        match goal with H: mfby _ _ _ _ _ _ |- _ => destruct H as (?&?) end; auto.
+    - specialize (Closed 0); destruct Closed as [? Vals].
+      intros ** Find.
+      assert (In x (SynNL.gather_mem (n_eqs n))) as Hin
+          by (apply Vals, not_None_is_Some; eauto).
+      destruct n; simpl in *.
+      unfold gather_eqs in *.
+      clear - Hin Find Heqs.
+      revert Hin; generalize (@nil (ident * ident)).
+      induction n_eqs0 as [|[] ? IH]; simpl in *; intros; try contradiction;
+        inversion_clear Heqs as [|?? Heq]; inv Heq; eauto.
+      + destruct i; try discriminate; eauto.
+      + destruct i; try discriminate; eauto.
+      + destruct Hin.
+        * subst.
+          match goal with H: mfby _ _ _ _ _ _ |- _ => destruct H as (Find'&?) end.
+          rewrite Find in Find'; inv Find'.
+          exists c0; split; auto.
+          apply In_fst_fold_left_gather_eq; left; left; auto.
+        * edestruct IH as (c1 &?& Hin); eauto.
+          exists c1; split; auto.
+          apply In_fst_fold_left_gather_eq; right; eauto.
   Qed.
 
   Lemma msem_eqs_In_snd_gather_eqs_spec:
@@ -162,7 +163,7 @@ Module Type CORRECTNESS
     induction eqs as [|[]]; simpl; intros ** Heqs Hin;
       inversion_clear Heqs as [|?? Heq];
       try inversion_clear Heq as [|????????????? Hd|???????????????? Hd|];
-        try contradiction; eauto.
+      try contradiction; eauto.
     - destruct i; try discriminate.
       apply In_snd_fold_left_gather_eq in Hin as [Hin|]; eauto.
       destruct Hin as [E|]; try contradiction; inv E; inv Hd.
@@ -172,6 +173,39 @@ Module Type CORRECTNESS
       destruct Hin as [E|]; try contradiction; inv E; inv Hd.
       do 4 eexists; split; eauto.
   Qed.
+
+  (* Lemma msem_eqs_In_snd_gather_eqs_spec': *)
+  (*   forall eqs G bk H M M' x f Mx_n n, *)
+  (*     Forall (msem_equation G bk H M M') eqs -> *)
+  (*     memory_closed_n M eqs -> *)
+  (*     sub_inst x (M n) Mx_n -> *)
+  (*     exists xss Mx Mx' yss, *)
+  (*       Mx n = Mx_n *)
+  (*       /\ (msem_node G f xss Mx Mx' yss *)
+  (*        \/ exists r, msem_reset G f r xss Mx Mx' yss) *)
+  (*       /\ In (x, f) (snd (gather_eqs eqs)). *)
+  (* Proof. *)
+  (*   unfold gather_eqs. *)
+  (*   intros. *)
+  (*   unfold memory_closed_n, memory_closed, sub_inst in *. *)
+  (*   assert (InMembers x (gather_insts eqs *)
+  (*   eapply H1 in H2.  *)
+  (*   intro; generalize (@nil (ident * const)). *)
+  (*   induction eqs as [|[]]; simpl; intros ** Heqs Hin; *)
+  (*     inversion_clear Heqs as [|?? Heq]; *)
+  (*     try inversion_clear Heq as [|????????????? Hd|???????????????? Hd|]; *)
+  (*     try contradiction; eauto. *)
+  (*   - *)
+  (*   - destruct i; try discriminate. *)
+  (*     apply In_snd_fold_left_gather_eq in Hin as [Hin|]; eauto. *)
+  (*     destruct Hin as [E|]; try contradiction; inv E; inv Hd. *)
+  (*     do 4 eexists; split; eauto. *)
+  (*   - destruct i; try discriminate. *)
+  (*     apply In_snd_fold_left_gather_eq in Hin as [Hin|]; eauto. *)
+  (*     destruct Hin as [E|]; try contradiction; inv E; inv Hd. *)
+  (*     do 4 eexists; split; eauto. *)
+  (* Qed. *)
+  (* Admitted. *)
 
   Lemma msem_node_initial_state:
     forall G f xss M M' yss,
@@ -184,7 +218,7 @@ Module Type CORRECTNESS
       match goal with Hf: find_node _ [] = _ |- _ => inversion Hf end.
     intros ** Hord Hsem.
     assert (Hsem' := Hsem).
-    inversion_clear Hsem' as [???????? Clock Hfind Ins ????? Heqs].
+    inversion_clear Hsem' as [???????? Clock Hfind Ins ????? Heqs Closed].
     pose proof (find_node_not_Is_node_in _ _ _ Hord Hfind) as Hnini.
     pose proof Hord; inversion_clear Hord as [|??? NodeIn].
     pose proof Hfind as Hfind'.
@@ -201,11 +235,11 @@ Module Type CORRECTNESS
       econstructor; eauto.
       + eapply msem_eqs_reset_lasts; eauto.
       + intros ** Hin.
-        assert (b' <> n_name node).
-        { destruct node; simpl in *.
-          apply In_snd_gather_eqs_Is_node_in in Hin.
-          apply NodeIn; auto.
-        }
+        (* assert (b' <> n_name node). *)
+        (* { destruct node; simpl in *. *)
+        (*   apply In_snd_gather_eqs_Is_node_in in Hin. *)
+        (*   apply NodeIn; auto. *)
+        (* } *)
         destruct node; simpl in *.
         edestruct msem_eqs_In_snd_gather_eqs_spec
           as (?& Mx &?&?& [Node|(rs & Reset)] & Sub); eauto.
@@ -215,6 +249,25 @@ Module Type CORRECTNESS
         specialize (Mmask 0); specialize (Sub 0).
         rewrite <-Mmask in Sub; auto.
         eexists; split; eauto.
+      + intros ** Sub.
+        assert (InMembers x (gather_insts (n_eqs node))) as Hin
+            by (apply (Closed 0); rewrite Sub; discriminate).
+        rewrite <-gather_eqs_snd_spec in Hin.
+        apply InMembers_In in Hin as (?&?).
+        destruct node; simpl in *.
+        edestruct msem_eqs_In_snd_gather_eqs_spec
+          as (?& Mx &?&?& [Node|(rs & Reset)] & Hin'); eauto.
+        * eexists; split; eauto.
+          specialize (Hin' 0); unfold sub_inst in *.
+          rewrite Sub in Hin'; inv Hin'; eauto.
+        * inversion_clear Reset as [?????? Nodes].
+          destruct (Nodes (count rs 0)) as (M0 &?& Node & Mmask &?).
+          apply IH in Node; auto.
+          specialize (Mmask 0).
+          eexists; split; eauto.
+          specialize (Hin' 0); unfold sub_inst in *.
+          rewrite Sub in Hin'; inv Hin'; eauto.
+          rewrite <-Mmask; eauto.
     - assert (n_name node <> f) by now apply ident_eqb_neq.
       eapply msem_node_cons in Hsem; eauto.
       simpl; rewrite <-initial_state_tail; eauto.
